coq_session/proc_step.v
@@ -1,0 +1,136 @@
+From mathcomp Require Import ssreflect ssrbool eqtype ssrnat seq.
+From Coq Require Import ssrfun Classical Utf8.
+Require Export AutosubstSsr ARS dyn_weak.
+
+Set Implicit Arguments.
+Unset Strict Implicit.
+Unset Printing Implicit Defensive.
+
+Inductive proc :=
+| Exp (m : term)
+| Par (p q : proc)
+| Nu (p : proc).
+
+Notation "⟨ m ⟩" := (Exp m).
+Notation "p ∣ q" := (Par p q) (at level 50).
+Notation "'ν.' p" := (Nu p) (at level 50).
+
+
+Lemma dyn_crename Θ Θ' Γ Γ' Δ Δ' m A ξ :
+  Θ ; Γ ; Δ ⊢ m : A -> dyn_agree_cren ξ Θ Γ Δ Θ' Γ' Δ' ->
+  Θ' ; Γ' ; Δ' ⊢ term_cren m ξ : term_cren A ξ.
+Proof with eauto using dyn_empty, dyn_type.
+  move=>ty. elim: ty Θ' Γ' Δ' ξ=>/={Θ Γ Δ m A}.
+  { intros.
+    econstructor.
+    admit.
+    admit.
+    admit.
+    admit. }
+  { intros.
+    econstructor.
+    admit.
+    admit.
+    apply: H2.
+    econstructor.
+    eauto.
+    admit.
+    eauto. }
+  { intros.
+    econstructor.
+    admit.
+    admit.
+    apply: H2.
+    constructor.
+    eauto.
+    admit.
+    eauto. }
+  { intros.
+    rewrite term_cren_beta.
+    apply: dyn_app0...
+    admit. }
+  { intros.
+    rewrite term_cren_beta.
+    apply: dyn_app1...
+    admit.
+    admit.
+    apply: H2.
+    admit.
+    apply: H4.
+    admit. }
+
+Lemma dyn_strengthen Θ m A :
+  _: Θ ; nil ; nil ⊢ term_cren m (+1) : term_cren A (+1) ->
+  Θ ; nil ; nil ⊢ m : A.
+Proof with eauto using dyn_empty, dyn_type.
+  intros.
+  replace m with (term_cren (term_cren m (+1)) (subn^~ 1)).
+  replace A with (term_cren (term_cren A (+1)) (subn^~ 1)).
+  apply: dyn_crename.
+  apply: H.
+  constructor.
+  replace (subn^~ 1) with (id >>> subn^~ 1) by autosubst.
+  constructor.
+  constructor.
+
+
+  move=>ty. elim: ty Γ' Δ'=>//={Θ Γ Δ m A}...
+  admit.
+  { intros.
+    constructor...
+    admit.
+    admit.
+    apply: H2.
+    econstructor...
+    admit. }
+  admit.
+  admit.
+  admit.
+  admit.
+  admit.
+  admit.
+  admit.
+  admit.
+  admit.
+  admit.
+  admit.
+  admit.
+  admit.
+  { intros.
+    replace (term_cren A.[ren (+size Γ)] (+1))
+      with (term_cren A (+1)).[ren (+size Γ')].
+    apply: dyn_cvar.
+    admit.
+    admit.
+    admit.
+    admit.
+    admit. }
+  { intros.
+    econstructor...
+    constructor... }
+  { intros.
+    econstructor...
+    constructor... }
+  { intros.
+  }
+Admitted.
+
+Lemma dyn_cweaken0 Θ m A :
+  Θ ; nil ; nil ⊢ m : A ->
+  _: Θ ; nil ; nil ⊢ term_cren m (+1) : term_cren A (+1).
+Proof with eauto using dyn_empty, dyn_type.
+  intros.
+  apply: dyn_cweaken...
+  constructor.
+
+  move=>ty. elim: ty Γ' Δ'=>//={Θ Γ Δ m A}...
+  { intros.
+    econstructor...
+
+    
+    constructor... }
+  { intros.
+    econstructor...
+    constructor... }
+  { intros.
+  }
