coq_session/sta_cren.v
@@ -1,0 +1,133 @@
+From mathcomp Require Import ssreflect ssrbool eqtype ssrnat seq.
+From Coq Require Import ssrfun Classical Utf8.
+Require Export AutosubstSsr ARS tll_cren sta_type.
+
+Set Implicit Arguments.
+Unset Strict Implicit.
+Unset Printing Implicit Defensive.
+
+Inductive sta_agree_cren : (nat -> nat) -> sta_ctx -> sta_ctx -> Prop :=
+| sta_agree_cren_nil ξ :
+  sta_agree_cren ξ nil nil
+| sta_agree_cren_cons Γ Γ' ξ m m' s :
+  m' = term_cren m ξ ->
+  Γ ⊢ m : Sort s ->
+  sta_agree_cren ξ Γ Γ' ->
+  sta_agree_cren ξ (m :: Γ) (m' :: Γ').
+
+Lemma sta_agree_cren_size Γ Γ' ξ :
+  sta_agree_cren ξ Γ Γ' -> size Γ = size Γ'.
+Proof with eauto.
+  elim=>{Γ Γ' ξ}...
+  move=>Γ Γ' ξ m m' s e1 tym agr e2=>//=.
+  by rewrite e2.
+Qed.
+
+Lemma sta_agree_cren_has Γ Γ' ξ x A :
+  sta_agree_cren ξ Γ Γ' ->
+  sta_has Γ x A ->
+  sta_has Γ' x (term_cren A ξ).
+Proof with eauto.
+  move=>agr. elim: agr x A=>{Γ Γ' ξ}.
+  { move=>ξ x A shs. inv shs. }
+  { move=>Γ Γ' ξ m m' s e tym agr ih x A shs. subst.
+    inv shs.
+    { rewrite term_cren_ren.
+      constructor. }
+    { rewrite term_cren_ren.
+      constructor... } }
+Qed.
+
+Lemma sta_crename Γ Γ' m A ξ :
+  Γ ⊢ m : A -> sta_agree_cren ξ Γ Γ' ->
+  Γ' ⊢ term_cren m ξ : term_cren A ξ.
+Proof with eauto using sta_type, sta_agree_cren.
+  move=>ty. move:Γ m A ty Γ' ξ.
+  apply:(@sta_type_mut _ (fun Γ wf => forall Γ' ξ, sta_agree_cren ξ Γ Γ' -> sta_wf Γ')); simpl...
+  { move=>Γ x A wf ih shs Γ' ξ agr.
+    constructor...
+    apply: sta_agree_cren_has... }
+  { move=>Γ A B m s tym ihm Γ' ξ agr.
+    have wf:=sta_type_wf tym. inv wf.
+    econstructor.
+    apply: ihm.
+    econstructor... }
+  { move=>Γ A B m s tym ihm Γ' ξ agr.
+    have wf:=sta_type_wf tym. inv wf.
+    econstructor.
+    apply: ihm.
+    econstructor... }
+  { move=>Γ A B m n s tym ihm tyn ihn Γ' ξ agr.
+    rewrite term_cren_beta1.
+    apply: sta_app0... }
+  { move=>Γ A B m n s tym ihm tyn ihn Γ' ξ agr.
+    rewrite term_cren_beta1.
+    apply: sta_app1... }
+  { move=>Γ A B m n t tyS ihS tym ihm tyn ihn Γ' ξ agr.
+    apply: sta_pair0...
+    rewrite<-term_cren_beta1... }
+  { move=>Γ A B m n t tyS ihS tym ihm tyn ihn Γ' ξ agr.
+    apply: sta_pair1...
+    rewrite<-term_cren_beta1... }
+  { move=>Γ A B C m n s t tyC ihC tym ihm tyn ihn Γ' ξ agr.
+    have wf:=sta_type_wf tyC. inv wf.
+    have wf:=sta_type_wf tyn. inv wf. inv H3.
+    rewrite term_cren_beta1.
+    apply: sta_letin0...
+    apply: ihC...
+    rewrite<-(term_cren_subst _ (term_csubst_pair0 ξ t)).
+    apply: ihn... }
+  { move=>Γ A B C m n s t tyC ihC tym ihm tyn ihn Γ' ξ agr.
+    have wf:=sta_type_wf tyC. inv wf.
+    have wf:=sta_type_wf tyn. inv wf. inv H3.
+    rewrite term_cren_beta1.
+    apply: sta_letin1...
+    apply: ihC...
+    rewrite<-(term_cren_subst _ (term_csubst_pair1 ξ t)).
+    apply: ihn... }
+  { move=>Γ A m tym ihm Γ' ξ agr.
+    have wf:=sta_type_wf tym. inv wf.
+    constructor.
+    rewrite<-term_cren_ren.
+    apply: ihm... }
+  { move=>Γ A m n1 n2 s tyA ihA tym ihm tyn1 ihn1 tyn2 ihn2 Γ' ξ
+           agr.
+    rewrite term_cren_beta1.
+    apply: sta_ifte...
+    replace TT with (term_cren TT ξ) by eauto.
+    rewrite<-term_cren_beta1...
+    replace FF with (term_cren FF ξ) by eauto.
+    rewrite<-term_cren_beta1... }
+  { move=>Γ m n A B s tyB ihB tym ihm tyn ihn Γ' ξ agr.
+    have wf:=sta_type_wf tyn. inv wf.
+    apply: sta_bind...
+    rewrite<-term_cren_ren... }
+  { move=>Γ r A B tyB ihB Γ' ξ agr.
+    have wf:=sta_type_wf tyB. inv wf.
+    apply: sta_act0. apply: ihB... }
+  { move=>Γ r A B tyB ihB Γ' ξ agr.
+    have wf:=sta_type_wf tyB. inv wf.
+    apply: sta_act1. apply: ihB... }
+  { move=>Γ r x A wf ih tyA ihA Γ' ξ agr.
+    rewrite term_cren_ren.
+    rewrite (sta_agree_cren_size agr).
+    apply: sta_cvar... }
+  { move=>Γ m A tym ihm Γ' ξ agr.
+    have wf:=sta_type_wf tym. inv wf.
+    constructor... }
+  { move=>Γ A B m s eq tym ihm tyB ihB Γ' ξ agr.
+    apply: sta_conv.
+    apply: term_cren_sta_conv...
+    apply: ihm...
+    apply: ihB... }
+  { move=>Γ' ξ agr. inv agr. constructor. }
+  { move=>Γ A s wf ih tyA ihA Γ' ξ agr. inv agr.
+    econstructor... }
+Qed.
+
+Lemma sta_ecrename Γ Γ' m m' A A' ξ :
+  m' = term_cren m ξ ->
+  A' = term_cren A ξ ->
+  Γ ⊢ m : A -> sta_agree_cren ξ Γ Γ' ->
+  Γ' ⊢ m' : A'.
+Proof. move=>->->. apply: sta_crename. Qed.
